src/SlabsUtils.fst
@@ -1,7 +1,10 @@
 module SlabsUtils
 
+module STU = SizeTUtils
+module US = FStar.SizeT
 module U64 = FStar.UInt64
 module U32 = FStar.UInt32
+module U16 = FStar.UInt16
 module U8 = FStar.UInt8
 
 module G = FStar.Ghost
@@ -20,7 +23,7 @@ open Utils
 open Utils2
 open SteelUtils
 
-#push-options "--z3rlimit 20"
+#push-options "--z3rlimit 30"
 let slot_array (size_class: sc) (arr: array U8.t) (pos: U32.t)
   : Pure (array U8.t)
   (requires
@@ -33,8 +36,12 @@ let slot_array (size_class: sc) (arr: array U8.t) (pos: U32.t)
   =
   let ptr = A.ptr_of arr in
   let shift = U32.mul pos size_class in
-  assert (U32.v shift < A.length arr);
-  let ptr_shifted = A.ptr_shift ptr shift in
+  nb_slots_correct size_class pos;
+  assert (U32.v shift <= U32.v page_size);
+  assert_norm (U32.v shift <= FStar.Int.max_int U16.n);
+  let shift_size_t = STU.small_uint32_to_sizet shift in
+  assert (US.v shift_size_t < A.length arr);
+  let ptr_shifted = A.ptr_shift ptr shift_size_t in
   (| ptr_shifted, G.hide (U32.v size_class) |)
 #pop-options
 
@@ -63,8 +70,10 @@ let array_slot_slot_array_bij (size_class: sc) (arr: array U8.t) (pos: U32.t)
   =
   let ptr = A.ptr_of arr in
   let shift = U32.mul pos size_class in
-  assert (U32.v shift < A.length arr);
-  let ptr_shifted = A.ptr_shift ptr shift in
+  nb_slots_correct size_class pos;
+  let shift_size_t = STU.small_uint32_to_sizet shift in
+  assert (US.v shift_size_t < A.length arr);
+  let ptr_shifted = A.ptr_shift ptr shift_size_t in
   let slot_as_array = slot_array size_class arr pos in
   assert (A.ptr_of slot_as_array == ptr_shifted);
   let offset_bytes = A.offset ptr_shifted - A.offset ptr in
@@ -76,141 +85,36 @@ let array_slot_slot_array_bij (size_class: sc) (arr: array U8.t) (pos: U32.t)
   let slot_as_pos = array_slot size_class arr slot_as_array in
   assert (G.reveal slot_as_pos == offset_slot)
 
-let slab_vprop1 (size_class: sc) (arr: array U8.t{A.length arr = U32.v page_size})
-  (s: Seq.seq (r:nat{r < U32.v (nb_slots size_class)}))
-  : GTot (Seq.seq vprop)
+let slot_vprop
+  (size_class: sc)
+  (arr: array U8.t{A.length arr = U32.v page_size})
+  (pos: nat{pos < U32.v (nb_slots size_class)})
   =
-  let f = fun (k:nat{k < U32.v (nb_slots size_class)})
-    -> A.varray (slot_array size_class arr (U32.uint_to_t k)) in
-  Seq.map_seq_len f s;
-  let s' = Seq.map_seq f s in
-  s'
+  A.varray (slot_array size_class arr (U32.uint_to_t pos))
 
-let slab_vprop2 (size_class: sc) (arr: array U8.t{A.length arr = U32.v page_size})
-  (s: Seq.seq (r:nat{r < U32.v (nb_slots size_class)}))
-  : GTot (list vprop)
+let slab_vprop_aux
+  (size_class: sc)
+  (arr: array U8.t{A.length arr = U32.v page_size})
+  (md_as_seq: Seq.lseq U64.t 4)
+  : vprop
   =
-  let s' = slab_vprop1 size_class arr s in
-  let r = Seq.seq_to_list s' in
-  r
-
-let slab_vprop3 (size_class: sc) (arr: array U8.t{A.length arr = U32.v page_size})
-  (s: Seq.seq (r:nat{r < U32.v (nb_slots size_class)}))
-  : GTot vprop
-  =
-  let r = slab_vprop2 size_class arr s in
-  starl r
-
-let slab_vprop2_lemma
-  (size_class: sc) (arr: array U8.t{A.length arr = U32.v page_size})
-  (s1 s2: Seq.seq (r:nat{r < U32.v (nb_slots size_class)}))
-  : Lemma
-  (slab_vprop2 size_class arr (Seq.append s1 s2)
-  == L.append (slab_vprop2 size_class arr s1) (slab_vprop2 size_class arr s2))
-  =
-  let f = fun (k:nat{k < U32.v (nb_slots size_class)})
-    -> A.varray (slot_array size_class arr (U32.uint_to_t k)) in
-  Seq.map_seq_append f s1 s2;
-  assert (
-     slab_vprop1 size_class arr (Seq.append s1 s2)
-  == Seq.append (slab_vprop1 size_class arr s1) (slab_vprop1 size_class arr s2));
-  lemma_seq_to_list_append
-    (slab_vprop1 size_class arr s1)
-    (slab_vprop1 size_class arr s2)
-
-let slab_vprop3_lemma
-  (size_class: sc) (arr: array U8.t{A.length arr = U32.v page_size})
-  (s1 s2: Seq.seq (r:nat{r < U32.v (nb_slots size_class)}))
-  : Lemma
-  (slab_vprop3 size_class arr (Seq.append s1 s2)
-  `equiv` (
-         (slab_vprop3 size_class arr s1)
-  `star` (slab_vprop3 size_class arr s2)))
-  =
-  let l1 = slab_vprop2 size_class arr s1 in
-  let l2 = slab_vprop2 size_class arr s2 in
-  slab_vprop2_lemma size_class arr s1 s2;
-  starl_append l1 l2
+  let incr_seq = SeqUtils.init_u32_refined (U32.v (nb_slots size_class))
+  in
+  let f = fun (i: U32.t{U32.v i < U32.v (nb_slots size_class)}) ->
+    if Bitmap4.get md_as_seq i
+    then slot_vprop size_class arr (U32.v i)
+    else emp
+  in
+  Seq.map_seq_len f incr_seq;
+  let vprop_seq
+    : Seq.lseq vprop (U32.v (nb_slots size_class))
+    = Seq.map_seq f incr_seq in
+  let vprop_list = Seq.seq_to_list vprop_seq in
+  starl vprop_list
 
 let slab_vprop
   (size_class: sc)
   (arr: array U8.t{A.length arr = U32.v page_size})
-  (i:nat)
-  (j:nat{i <= j /\ j <= U32.v (nb_slots size_class)})
-  : Tot vprop
-  =
-  let s = Seq.slice (Seq.init (U32.v (nb_slots size_class)) (fun k -> k)) i j in
-  slab_vprop3 size_class arr s
-
-let slab_vprop_lemma
-  (size_class: sc)
-  (arr: array U8.t{A.length arr = U32.v page_size})
-  (i:nat)
-  (j:nat{i <= j /\ j <= U32.v (nb_slots size_class)})
-  (k:nat{i <= k /\ k <= j})
-  : Lemma
-  (slab_vprop size_class arr i j
-  `equiv` (
-         (slab_vprop size_class arr i k)
-  `star` (slab_vprop size_class arr k j)))
-  =
-  let s = Seq.init (U32.v (nb_slots size_class)) (fun k -> k) in
-  let s1 = Seq.slice s i j in
-  let s2, s3 = Seq.split s1 (k - i) in
-  Seq.lemma_split s1 (k - i);
-  assert (s2 == Seq.slice s1 0 (k - i));
-  Classical.forall_intro (lemma_index_slice s1 0 (k - i));
-  assert (s3 == Seq.slice s1 (k - i) (j - i));
-  Classical.forall_intro (lemma_index_slice s1 (k - i) (j - i));
-  slab_vprop3_lemma size_class arr s2 s3
-
-
-let slab_vprop_sl_lemma
-  (size_class: sc)
   (md: slab_metadata)
-  (arr: array U8.t{A.length arr = U32.v page_size})
-  (i:nat)
-  (j:nat{i <= j /\ j <= U32.v (nb_slots size_class)})
-  (k:nat{i <= k /\ k <= j})
-  (m: SM.mem)
-  : Lemma
-  (requires SM.interp (hp_of (
-    (slab_vprop size_class arr i j)
-  )) m)
-  (ensures SM.interp (hp_of (
-    (slab_vprop size_class arr i k `star`
-    slab_vprop size_class arr k j)
-  )) m)
   =
-  slab_vprop_lemma size_class arr i j k;
-  let p = slab_vprop size_class arr i j in
-  let q = (slab_vprop size_class arr i k) `star`
-          (slab_vprop size_class arr k j) in
-  assert (p `equiv` q);
-  reveal_equiv p q;
-  assert (hp_of p `SM.equiv` hp_of q);
-  SM.reveal_equiv (hp_of p) (hp_of q)
-
-let slab_vprop_singleton_lemma
-  (size_class: sc)
-  (arr: array U8.t{A.length arr = U32.v page_size})
-  (pos: U32.t{0 <= (U32.v pos) /\ (U32.v pos) < U32.v (nb_slots size_class)})
-  : Lemma
-  (slab_vprop size_class arr (U32.v pos) (U32.v pos + 1)
-  ==
-  (A.varray (slot_array size_class arr pos) `star` emp)
-  )
-  =
-  let r = slab_vprop size_class arr (U32.v pos) (U32.v pos + 1) in
-  let s = Seq.slice (Seq.init (U32.v (nb_slots size_class)) (fun k -> k))
-    (U32.v pos) (U32.v pos + 1) in
-  assert (r == slab_vprop3 size_class arr s);
-  assert (r == starl (slab_vprop2 size_class arr s));
-  assert (r == starl (Seq.seq_to_list (slab_vprop1 size_class arr s)));
-  let f = fun (k:nat{k < U32.v (nb_slots size_class)})
-    -> A.varray (slot_array size_class arr (U32.uint_to_t k)) in
-  Seq.map_seq_len f s;
-  assert (Seq.length (slab_vprop1 size_class arr s) == 1);
-  Seq.map_seq_index f s 0;
-  assert (r == starl ([A.varray (slot_array size_class arr pos)]));
-  assert (r == A.varray (slot_array size_class arr pos) `star` emp)
+  A.varray md `vdep` (fun md_as_seq -> slab_vprop_aux size_class arr md_as_seq)
