lib_misc/SeqUtils.fst
@@ -1,0 +1,44 @@
+module SeqUtils
+
+module U32 = FStar.UInt32
+
+noextract
+let init_nat (len: nat)
+  : Seq.lseq (k:nat{k < len}) len
+  = Seq.init len (fun k -> k)
+
+let init_nat_index (len: nat) (i:nat{i < len})
+  : Lemma
+  (Seq.index (init_nat len) i = i)
+  = ()
+
+noextract
+let init_nat_refined (len: nat) (len2: nat)
+  : Pure (Seq.lseq (k:nat{k < len2}) len)
+  (requires len <= len2)
+  (ensures fun _ -> True)
+  =
+  let s : Seq.lseq (k:nat{k < len}) len
+    = Seq.init len (fun k -> k) in
+  let f : (k:nat{k < len}) -> (k':nat{k' < len2})
+    = fun k -> k in
+  Seq.map_seq_len f s;
+  let s' : Seq.lseq (k:nat{k < len2}) len
+    = Seq.map_seq f s in
+  s'
+
+noextract
+let init_u32_refined (len: nat)
+  : Pure (Seq.lseq (k:U32.t{U32.v k < len}) len)
+  (requires FStar.UInt.size len U32.n)
+  (ensures fun _ -> True)
+  =
+  let s : Seq.lseq (k:nat{k < len}) len
+    = Seq.init len (fun k -> k) in
+  let f : (k:nat{k < len}) -> (k':U32.t{U32.v k' < len})
+    = fun k -> U32.uint_to_t k in
+  Seq.map_seq_len f s;
+  let s' : Seq.lseq (k:U32.t{U32.v k < len}) len
+    = Seq.map_seq f s in
+  s'
+
